src/semantics.lean
@@ -1,6 +1,11 @@
-import .hol data.bool
+/-
+Copyright (c) 2018 Jeremy Avigad. All rights reserved.
+Released under Apache 2.0 license as described in the file LICENSE.
+Authors: Jeremy Avigad
 
-universe u
+The "standard" semantics for type theory: `type`s denote `Type`s, and `terms` denote values of the corresponding types.
+-/
+import .syntax data.bool
 
 /- For now, we're only dealing with "pure" types, i.e. types without type
    variables and constructors -- only basic types and arrows.
@@ -43,7 +48,7 @@ def ok (bval : ℕ → option Type*) : type.basic → _root_.bool
 
 def eval (bval : ℕ → option Type*) : Π b : type.basic, b.ok bval = tt → Type*
 | (user n) h := option.get h
-| prop     h := _root_.bool
+| prop     h := Prop
 | nat      h := _root_.nat
 | bool     h := _root_.bool
 | int      h := _root_.int
@@ -77,9 +82,26 @@ def eval (bval : ℕ → option Type*) : Π t : type, t.ok bval → Type*
 | (Constructor _) h := by { simp [type.ok] at h, contradiction }
 | (App _ _ )      h := by { simp [type.ok] at h, contradiction }
 
+/- some useful functions -/
+theorem ok_domain (bval : ℕ → option Type*): Π t : type, t.ok bval → t.domain.ok bval :=
+begin
+  intro t, induction t; try {exact id}, 
+  simp [type.domain, type.ok], intro h, exact h.left
+end
+
+theorem ok_codomain (bval : ℕ → option Type*): Π t : type, t.ok bval → t.codomain.ok bval :=
+begin
+  intro t, induction t; try {exact id}, 
+  simp [type.codomain, type.ok], intro h, exact h.right
+end
+
+def eval_ext (bval : ℕ → option Type*) (t₁ t₂: type) (h : t₁ = t₂) : 
+  ∀ h₁ h₂, t₁.eval bval h₁ = t₂.eval bval h₂ :=
+by { rw h, intros, reflexivity }
+
 end type
 
-/- For the moment, only closed terms, no quantifiers -/
+/- We can use these to interpret quantifiers with bool in place of Prop.
 
 section
 local attribute [instance] classical.prop_decidable
@@ -91,6 +113,7 @@ noncomputable def classical_bex (T : Type*) (f : T → bool) : bool :=
 if ∃ t : T, f t = bool.tt then bool.tt else bool.ff
 
 end
+-/
 
 namespace term
 
@@ -100,23 +123,23 @@ inductive evaluates_to (bval : ℕ → option Type*) (cval : ℕ → option (Σ 
   const → Π T : Type*, T → Prop
 | eval_user (n : ℕ) (h : option.is_some (cval n)) (t : hol.type) (l : list hol.type) : 
     evaluates_to ⟨kind.user n, t, l⟩ (option.get h).1 (option.get h).2
-| eval_true  : evaluates_to ⟨kind.true, mk_prop, []⟩ bool bool.tt
-| eval_false : evaluates_to ⟨kind.false, mk_prop, []⟩ bool bool.ff
-| eval_not   : evaluates_to ⟨kind.not, mk_prop ⇒ mk_prop, []⟩ (bool → bool) bnot
-| eval_and   : evaluates_to ⟨kind.and, mk_prop ⇒ mk_prop ⇒ mk_prop, []⟩ (bool → bool → bool) band
-| eval_or    : evaluates_to ⟨kind.or, mk_prop ⇒ mk_prop ⇒ mk_prop, []⟩ (bool → bool → bool) bor
+| eval_true  : evaluates_to ⟨kind.true, mk_prop, []⟩ Prop _root_.true
+| eval_false : evaluates_to ⟨kind.false, mk_prop, []⟩ Prop _root_.false
+| eval_not   : evaluates_to ⟨kind.not, mk_prop ⇒ mk_prop, []⟩ (Prop → Prop) (λ P, ¬ P)
+| eval_and   : evaluates_to ⟨kind.and, mk_prop ⇒ mk_prop ⇒ mk_prop, []⟩ (Prop → Prop → Prop) _root_.and
+| eval_or    : evaluates_to ⟨kind.or, mk_prop ⇒ mk_prop ⇒ mk_prop, []⟩ (Prop → Prop → Prop) _root_.or
 | eval_implies : evaluates_to ⟨kind.implies, mk_prop ⇒ mk_prop ⇒ mk_prop, []⟩ 
-                    (bool → bool → bool) (λ b₁ b₂, bor (bnot b₁) b₂)
+                    (Prop → Prop → Prop) (λ P Q, P → Q)
 | eval_iff   : evaluates_to ⟨kind.iff, mk_prop ⇒ mk_prop ⇒ mk_prop, []⟩ 
-                    (bool → bool → bool) (λ b₁ b₂, if b₁ = b₂ then bool.tt else bool.ff)
+                    (Prop → Prop → Prop) _root_.iff
 | eval_all (t : hol.type) (h : t.ok bval)  : 
                   let T := type.eval bval t h in
-                  evaluates_to ⟨kind.all, (t ⇒ mk_prop) ⇒ mk_prop, [t]⟩ ((T → bool) → bool)
-                    (classical_ball T)
+                  evaluates_to ⟨kind.all, (t ⇒ mk_prop) ⇒ mk_prop, [t]⟩ ((T → Prop) → Prop)
+                    (λ P, ∀ x : T, P x)
 | eval_ex  (t : hol.type) (h : t.ok bval)  : 
                   let T := type.eval bval t h in
-                  evaluates_to ⟨kind.all, (t ⇒ mk_prop) ⇒ mk_prop, [t]⟩ ((T → bool) → bool)
-                    (classical_bex T)
+                  evaluates_to ⟨kind.all, (t ⇒ mk_prop) ⇒ mk_prop, [t]⟩ ((T → Prop) → Prop)
+                    (λ P, ∃ x : T, P x)
 | eval_add   : evaluates_to ⟨kind.add, mk_nat ⇒ mk_nat ⇒ mk_nat, []⟩ (nat → nat → nat) nat.add
 | eval_mul   : evaluates_to ⟨kind.mul, mk_nat ⇒ mk_nat ⇒ mk_nat, []⟩ (nat → nat → nat) nat.mul
 | eval_sub   : evaluates_to ⟨kind.sub, mk_nat ⇒ mk_nat ⇒ mk_nat, []⟩ (nat → nat → nat) nat.sub
@@ -136,10 +159,10 @@ inductive ok (bval : ℕ → option Type*) (cval : ℕ → option (Σ T : Type*,
 | ok_or    : ok ⟨kind.or, mk_prop ⇒ mk_prop ⇒ mk_prop, []⟩
 | ok_implies : ok ⟨kind.implies, mk_prop ⇒ mk_prop ⇒ mk_prop, []⟩
 | ok_iff   : ok ⟨kind.iff, mk_prop ⇒ mk_prop ⇒ mk_prop, []⟩ 
---| ok_all (t : hol.type) (h : t.ok bval)  : 
---                  ok ⟨kind.all, (t ⇒ mk_prop) ⇒ mk_prop, [t]⟩
---| ok_ex  (t : hol.type) (h : t.ok bval)  : 
---                  ok ⟨kind.ex, (t ⇒ mk_prop) ⇒ mk_prop, [t]⟩
+| ok_all (t : hol.type) (h : t.ok bval)  : 
+                  ok ⟨kind.all, (t ⇒ mk_prop) ⇒ mk_prop, [t]⟩
+| ok_ex  (t : hol.type) (h : t.ok bval)  : 
+                  ok ⟨kind.ex, (t ⇒ mk_prop) ⇒ mk_prop, [t]⟩
 | ok_add   : ok ⟨kind.add, mk_nat ⇒ mk_nat ⇒ mk_nat, []⟩
 | ok_mul   : ok ⟨kind.mul, mk_nat ⇒ mk_nat ⇒ mk_nat, []⟩
 | ok_sub   : ok ⟨kind.sub, mk_nat ⇒ mk_nat ⇒ mk_nat, []⟩
@@ -148,58 +171,87 @@ inductive ok (bval : ℕ → option Type*) (cval : ℕ → option (Σ T : Type*,
 
 def type_ok (bval : ℕ → option Type*) (cval : ℕ → option (Σ T : Type*, T)) :
   ∀ c : const, c.ok bval cval → c.type.ok bval
-| ⟨kind.user n, t, l⟩ h := by cases h; assumption
-| ⟨kind.true, t, k⟩ h := by cases h; apply eq.refl 
-| ⟨kind.false, t, k⟩ h := by cases h; apply eq.refl 
-| ⟨kind.not, t, k⟩ h := by cases h; apply eq.refl 
-| ⟨kind.and, t, k⟩ h := by cases h; apply eq.refl 
-| ⟨kind.or, t, k⟩ h := by cases h; apply eq.refl 
+| ⟨kind.user n, t, l⟩ h  := by cases h; assumption
+| ⟨kind.true, t, k⟩ h    := by cases h; apply eq.refl 
+| ⟨kind.false, t, k⟩ h   := by cases h; apply eq.refl 
+| ⟨kind.not, t, k⟩ h     := by cases h; apply eq.refl 
+| ⟨kind.and, t, k⟩ h     := by cases h; apply eq.refl 
+| ⟨kind.or, t, k⟩ h      := by cases h; apply eq.refl 
 | ⟨kind.implies, t, k⟩ h := by cases h; apply eq.refl 
-| ⟨kind.iff, t, k⟩ h := by cases h; apply eq.refl 
-| ⟨kind.all, t, k⟩ h := by cases h; apply eq.refl 
-| ⟨kind.ex, t, k⟩ h := by cases h; apply eq.refl 
-| ⟨kind.add, t, k⟩ h := by cases h; apply eq.refl 
-| ⟨kind.mul, t, k⟩ h := by cases h; apply eq.refl 
-| ⟨kind.sub, t, k⟩ h := by cases h; apply eq.refl 
-| ⟨kind.bval b, t, k⟩ h := by cases h; apply eq.refl 
-| ⟨kind.nval n, t, k⟩ h := by cases h; apply eq.refl 
+| ⟨kind.iff, t, k⟩ h     := by cases h; apply eq.refl 
+| ⟨kind.all, t, k⟩ h     := 
+    begin 
+      cases k with ty k', 
+      cases h, 
+      cases k'; cases h, 
+      simp [type.ok, mk_prop, type.basic.ok], 
+      assumption 
+    end
+| ⟨kind.ex, t, k⟩ h     := 
+    begin 
+      cases k with ty k', 
+      cases h, 
+      cases k'; cases h, 
+      simp [type.ok, mk_prop, type.basic.ok], 
+      assumption 
+    end
+| ⟨kind.add, t, k⟩ h     := by cases h; apply eq.refl 
+| ⟨kind.mul, t, k⟩ h     := by cases h; apply eq.refl 
+| ⟨kind.sub, t, k⟩ h     := by cases h; apply eq.refl 
+| ⟨kind.bval b, t, k⟩ h  := by cases h; apply eq.refl 
+| ⟨kind.nval n, t, k⟩ h  := by cases h; apply eq.refl 
 
 def eval (bval : ℕ → option Type*) (cval : ℕ → option (Σ T : Type*, T)) : 
   Π (c : const) (h : c.ok bval cval), 
     (c.type).eval bval (c.type_ok bval cval h) 
 | c@⟨kind.user n, ty, l⟩ h := 
     have h' : option.is_some (cval n), by cases h; assumption,
-    have h'' :  c.type.eval bval (c.type_ok bval cval h)  = (option.get h').fst,
+    have h'' :  c.type.eval bval (c.type_ok bval cval h)  = (option.get h').fst, 
       by {cases h, assumption}, 
     cast h''.symm (option.get h').snd
-| c@⟨kind.true, _, _⟩     h := cast (by cases h; reflexivity) bool.tt 
-| c@⟨kind.false, _, _⟩    h := cast (by cases h; reflexivity) bool.tt 
-| c@⟨kind.not, _, _⟩      h := cast (by cases h; reflexivity) bnot  
-| c@⟨kind.and, _, _⟩      h := cast (by cases h; reflexivity) band
-| c@⟨kind.or, _, _⟩       h := cast (by cases h; reflexivity) bor
+| c@⟨kind.true, _, _⟩     h := cast (by cases h; reflexivity) _root_.true
+| c@⟨kind.false, _, _⟩    h := cast (by cases h; reflexivity) _root_.false
+| c@⟨kind.not, _, _⟩      h := 
+    have h' : (c.type).eval bval (c.type_ok bval cval h) = (Prop → Prop),
+      by cases h; reflexivity,
+    cast h'.symm (λ p : Prop, ¬ p)
+| c@⟨kind.and, _, _⟩      h := 
+    have h' : (c.type).eval bval (c.type_ok bval cval h) = (Prop → (Prop → Prop)),
+      by cases h; reflexivity,
+    cast h'.symm _root_.and
+| c@⟨kind.or, _, _⟩       h := 
+    have h' : (c.type).eval bval (c.type_ok bval cval h) = (Prop → (Prop → Prop)),
+      by cases h; reflexivity,
+    cast h'.symm _root_.or
 | c@⟨kind.implies, _, _⟩  h := 
-    have h' : c.type.eval bval (c.type_ok bval cval h) = (bool → bool → bool),
-      by {cases h, reflexivity}, 
-    cast h'.symm (λ b₁ b₂, bor (bnot b₁) b₂) 
+    have h' : (c.type).eval bval (c.type_ok bval cval h) = (Prop → (Prop → Prop)),
+      by cases h; reflexivity,
+    cast h'.symm (λ p q, p → q)
 | c@⟨kind.iff, _, _⟩      h := 
-    have h' : c.type.eval bval (c.type_ok bval cval h) = (bool → bool → bool),
-      by {cases h, reflexivity},
-    cast h'.symm (λ b₁ b₂, if b₁ = b₂ then bool.tt else bool.ff)
--- these are the noncomputable clauses 
---| ⟨kind.all, _, [t]⟩    h := have h' : t.ok bval, by cases h; assumption,
---                             let T := type.eval_safe bval t h' in
---                             ⟨((T → bool) → bool), (classical_ball T)⟩ 
---| ⟨kind.ex, _, [t]⟩     h := have h' : t.ok bval, by cases h; assumption,
---                             let T := type.eval_safe bval t h' in
---                             ⟨((T → bool) → bool), (classical_bex T)⟩ 
+    have h' : (c.type).eval bval (c.type_ok bval cval h) = (Prop → (Prop → Prop)),
+      by cases h; reflexivity,
+    cast h'.symm _root_.iff
+| c@⟨kind.all, _, [ty]⟩    h  :=
+    have h' : ty.ok bval, by cases h; assumption,
+    let T := ty.eval bval h' in
+    have h'' : (c.type).eval bval (c.type_ok bval cval h) = ((T → Prop) → Prop),
+      by cases h; reflexivity,
+    cast h''.symm (λ P, ∀ x : T, P x)
+| c@⟨kind.ex, _, [ty]⟩    h  :=
+    have h' : ty.ok bval, by cases h; assumption,
+    let T := ty.eval bval h' in
+    have h'' : (c.type).eval bval (c.type_ok bval cval h) = ((T → Prop) → Prop),
+      by cases h; reflexivity,
+    cast h''.symm Exists
 | c@⟨kind.add, _, _⟩      h := cast (by cases h; reflexivity) nat.add 
 | c@⟨kind.mul, _, _⟩      h := cast (by cases h; reflexivity) nat.mul 
 | c@⟨kind.sub, _, _⟩      h := cast (by cases h; reflexivity) nat.sub 
 | c@⟨kind.bval b, _, _⟩   h := cast (by cases h; reflexivity) b 
 | c@⟨kind.nval n, _, _⟩   h := cast (by cases h; reflexivity) n
-| c@⟨kind.all, _, _⟩      h := false.elim (by cases h)
-| c@⟨kind.ex, _, _⟩       h := false.elim (by cases h)
-
+| c@⟨kind.all, _, []⟩     h := false.elim (by cases h)
+| c@⟨kind.all, _, a :: b :: l⟩ h := false.elim (by cases h)
+| c@⟨kind.ex, _, []⟩     h := false.elim (by cases h)
+| c@⟨kind.ex, _, a :: b :: l⟩ h := false.elim (by cases h)
 
 /- TODO: prove that `evaluates_to` agrees with `eval`. -/ 
 
@@ -219,17 +271,6 @@ inductive evaluates_to (bval : ℕ → option Type*) (cval : ℕ → option (Σ 
     evaluates_to (term.Abs s ty t) σ (T₁ → T₂) f
 
 /-
-inductive ok (bval : ℕ → option Type*) (cval : ℕ → option (Σ T : Type*, T)) : 
-  term → list Type* → Prop
-| ok_var {n : ℕ} (σ : list Type*) {h : n < σ.length}      : ok (Var n) σ
-| ok_const {c : const} {σ} (h : c.well_typed bval cval)   : ok (Const c) σ
-| ok_app {t₁ t₂ : term} {σ} (h₁ : ok t₁ σ) (h₂ : ok t₂ σ) : ok (term.App t₁ t₂) σ
-| ok_abs {s : string} {ty : type} {t : term} {σ}  
-      (h₁ : ty.ok bval = tt) (h₂ : ok t (ty.eval_safe bval h₁ :: σ)) :
-    ok (term.Abs s ty t) σ
--/
-
-/-
 The reason it is so hard to write an evaluation function for a term is that there is
 so much data, and constraints. To evaluate a term `t`, we need
 
@@ -244,78 +285,11 @@ and we need to know:
   `bval` interprets all the relevant basic types
   `cval` interprets all the relevant constants, and assigns values of the right types
   `l` interprets all the relevant deBruin indices, and assigns values of the right types
+
+The next complicated predicate says that a term `t` is well-typed and we have the right
+data to interpret it.
 -/
 
--- TODO: move the next three
-def domain : type → type
-| (type.Arr t₁ t₂) := t₁
-| t                := t
-
-def codomain : type → type
-| (type.Arr t₁ t₂) := t₂ 
-| t                := t
-
-theorem ok_domain (bval : ℕ → option Type*): Π t : type, t.ok bval → (domain t).ok bval :=
-begin
-  intro t, induction t; try {exact id}, 
-  simp [domain, type.ok], intro h, exact h.left
-end
-
-theorem ok_codomain (bval : ℕ → option Type*): Π t : type, t.ok bval → (codomain t).ok bval :=
-begin
-  intro t, induction t; try {exact id}, 
-  simp [codomain, type.ok], intro h, exact h.right
-end
-
-inductive is_arrow : type → Prop
-| arr_is_arrow (t₁ t₂ : type) : is_arrow (t₁ ⇒ t₂)
-
-theorem eq_of_is_arrow (t : type) (h : is_arrow t) : t = (domain t ⇒ codomain t) :=
-by cases h; reflexivity
-
-inductive type_list_ok : term → list type → Prop
-| ok_var (n : nat) (σ : list type) (h : n < σ.length) : type_list_ok (Var n) σ
-| ok_const (c : const) (σ : list type)                : type_list_ok (Const c) σ
-| ok_app (t₁ t₂ : term) (σ : list type) 
-    (h₁ : type_list_ok t₁ σ) (h₂ : type_list_ok t₂ σ) : type_list_ok (App t₁ t₂) σ
-| ok_abs (s : string) (ty : type) (t : term) 
-    (σ : list type) (h : type_list_ok t (ty :: σ))    : type_list_ok (Abs s ty t) σ
-
-def typeof' : Π (t : term) (σ : list type), type_list_ok t σ → type
-| (Var n) σ h       := have h' : n < σ.length, by {cases h, assumption},
-                       σ.nth_le n h'
-| (Const c) σ h     := c.type
-| (App t₁ t₂) σ h   := have h' : type_list_ok t₁ σ, by {cases h, assumption}, 
-                       codomain (typeof' t₁ σ h')
-| (Abs s ty t) σ h  := have h' : type_list_ok t (ty :: σ), by {cases h, assumption},
-                       ty ⇒ typeof' t (ty :: σ) h'
-
-def typeof : term → list type → type
-| (Var n) σ       := if h : n < σ.length then σ.nth_le n h else mk_nat
-| (Const c) σ     := c.type
-| (App t₁ t₂) σ   := codomain (typeof t₁ σ)
-| (Abs s ty t) σ  := ty ⇒ typeof t (ty :: σ)
-
-inductive is_well_typed : term → list type → Prop
-| wt_var (n : ℕ) (σ : list type) (h : n < σ.length)      : is_well_typed (Var n) σ
-| wt_const (c : const) (σ : list type)                   : is_well_typed (Const c) σ
-| wt_app (t₁ t₂ : term) (σ : list type) 
-    (h₁ : is_well_typed t₁ σ) 
-    (h₂ : is_well_typed t₂ σ) 
-    (h₃ : is_arrow (typeof t₁ σ)) 
-    (h₄ : domain (typeof t₁ σ) = typeof t₂ σ)            : is_well_typed (App t₁ t₂) σ
-| wt_abs (s : string) (ty : type) (t : term) 
-      (σ : list type)
-    (h₁ : is_well_typed t (ty :: σ))                     : is_well_typed (Abs s ty t) σ
-
-
--- move
-def eval_ext (bval : ℕ → option Type*) (t₁ t₂: type) (h : t₁ = t₂) : 
-  ∀ h₁ h₂, t₁.eval bval h₁ = t₂.eval bval h₂ :=
-by { rw h, intros, reflexivity }
-
--- this complicated predicate says that a term `t` is well-typed and we have the right
--- data to interpret it
 inductive ok (bval : ℕ → option Type*) (cval : ℕ → option (Σ T : Type*, T)) : 
   Π (t : term) (σ : list type) (l : list (Σ T : Type*, T)), Prop
 | var_ok (n : nat) (σ : list type) (l : list (Σ T : Type*, T))
@@ -326,8 +300,8 @@ inductive ok (bval : ℕ → option Type*) (cval : ℕ → option (Σ T : Type*,
   ok (Const c) σ l
 | app_ok (t₁ t₂ : term) (σ : list type) (l : list (Σ T : Type*, T))
     (h₁ : ok t₁ σ l) (h₂ : ok t₂ σ l) 
-    (h₃ : is_arrow (typeof t₁ σ)) 
-    (h₄ : domain (typeof t₁ σ) = typeof t₂ σ):
+    (h₃ : (typeof t₁ σ).is_arrow) 
+    (h₄ : (typeof t₁ σ).domain = typeof t₂ σ):
   ok (App t₁ t₂) σ l
 | abs_ok (s : string) (ty : type) (t : term) (σ : list type) (l : list (Σ T : Type*, T)) 
     (h₀ : ty.ok bval)
@@ -348,7 +322,7 @@ def type_ok (bval : ℕ → option Type*) (cval : ℕ → option (Σ T : Type*, 
     c.type_ok bval cval h₀
 | (App t₁ t₂) σ l h :=
     have h₁ : t₁.ok bval cval σ l, by {cases h, assumption},
-    by { simp [typeof], apply ok_codomain, apply type_ok t₁ σ l, assumption}  
+    by { simp [typeof], apply type.ok_codomain, apply type_ok t₁ σ l, assumption}  
 | (Abs s ty t) σ l h := 
     by { simp [typeof, type.ok], cases h, split; assumption }
 
@@ -362,7 +336,7 @@ def eval (bval : ℕ → option Type*) (cval : ℕ → option (Σ T : Type*, T))
     have h₃ : (σ.nth_le n h₀).eval bval h₂ = (l.nth_le n h₁).fst, by cases h; assumption,
     have h₄ : (typeof (Var n) σ).eval bval ((Var n).type_ok bval cval σ l h) = 
         (l.nth_le n h₁).fst,
-      by { rw ← h₃, apply eval_ext, simp [typeof, h₀] },
+      by { rw ← h₃, apply type.eval_ext, simp [typeof, h₀] },
      cast h₄.symm (l.nth_le n h₁).snd 
 | (Const c) σ l h :=
     have h : c.ok bval cval, by cases h; assumption,
@@ -370,21 +344,21 @@ def eval (bval : ℕ → option Type*) (cval : ℕ → option (Σ T : Type*, T))
 | (App t₁ t₂) σ l h :=
     have h₁ : t₁.ok bval cval σ l, by cases h; assumption,
     have h₂ : t₂.ok bval cval σ l, by cases h; assumption,
-    have h₃ : is_arrow (typeof t₁ σ), by cases h; assumption,
-    have h₄ : domain (typeof t₁ σ) = typeof t₂ σ, by cases h; assumption,
-    have h₅ : typeof t₁ σ = (domain (typeof t₁ σ) ⇒ codomain (typeof t₁ σ)), from eq_of_is_arrow _ h₃,
+    have h₃ : (typeof t₁ σ).is_arrow, by cases h; assumption,
+    have h₄ : (typeof t₁ σ).domain = typeof t₂ σ, by cases h; assumption,
+    have h₅ : typeof t₁ σ = ((typeof t₁ σ).domain ⇒ (typeof t₁ σ).codomain), from type.eq_of_is_arrow _ h₃,
     have h₆ : (typeof t₁ σ).ok bval, from t₁.type_ok bval cval σ l h₁, 
-    have h₇ : (domain (typeof t₁ σ) ⇒ codomain (typeof t₁ σ)).ok bval, by rw ← h₅; exact h₆,
-    have h₈ : (typeof t₁ σ).eval bval h₆ = (domain (typeof t₁ σ) ⇒ codomain (typeof t₁ σ)).eval bval h₇,
-      from eval_ext bval _ _ h₅ _ _,
-    have h₉ : (domain (typeof t₁ σ)).ok bval, from ok_domain _ _ h₆,
-    have h₁₀ : (codomain (typeof t₁ σ)).ok bval, from ok_codomain _ _ h₆,
+    have h₇ : ((typeof t₁ σ).domain ⇒ (typeof t₁ σ).codomain).ok bval, by rw ← h₅; exact h₆,
+    have h₈ : (typeof t₁ σ).eval bval h₆ = ((typeof t₁ σ).domain ⇒ (typeof t₁ σ).codomain).eval bval h₇,
+      from type.eval_ext bval _ _ h₅ _ _,
+    have h₉ : (typeof t₁ σ).domain.ok bval, from type.ok_domain _ _ h₆,
+    have h₁₀ : (typeof t₁ σ).codomain.ok bval, from type.ok_codomain _ _ h₆,
     have h₁₁ : (typeof t₁ σ).eval bval h₆ =
-                  ((domain (typeof t₁ σ)).eval bval h₉ → (codomain (typeof t₁ σ)).eval bval h₁₀), 
+                  ((typeof t₁ σ).domain.eval bval h₉ → (typeof t₁ σ).codomain.eval bval h₁₀), 
       from h₈,
     have h₁₂ : (typeof t₂ σ).ok bval, from t₂.type_ok bval cval σ l h₂,
-    have h₁₃ : (typeof t₂ σ).eval bval h₁₂ = (domain (typeof t₁ σ)).eval bval h₉, 
-      from eval_ext bval _ _ h₄.symm _ _, 
+    have h₁₃ : (typeof t₂ σ).eval bval h₁₂ = (typeof t₁ σ).domain.eval bval h₉, 
+      from type.eval_ext bval _ _ h₄.symm _ _, 
     let  v₁ := eval t₁ σ l h₁,
          v₂ := eval t₂ σ l h₂ in
     (cast h₁₁ v₁) (cast h₁₃ v₂)
