src/examples.lean
@@ -1,0 +1,28 @@
+/-
+Copyright (c) 2018 Jeremy Avigad. All rights reserved.
+Released under Apache 2.0 license as described in the file LICENSE.
+Authors: Jeremy Avigad
+-/
+import .subst
+
+section examples
+
+open hol
+open hol.term
+
+private def foo : term :=
+  let ty := mk_nat ⇒ mk_nat ⇒ mk_nat,
+      f := Const (const.user 0 ty []),
+      x := Var 0,
+      y := Var 1,
+      t := abstract 1 "y" mk_nat (App (App f x) y),
+      c := Const (const.user 1 mk_nat []),
+      s := subst c 0 t in
+  s
+
+#eval foo.repr
+#eval repr (foo.typeof [])
+
+end examples
+
+
