src/syntax.lean
@@ -1,0 +1,615 @@
+/-
+Copyright (c) 2018 Jeremy Avigad. All rights reserved.
+Released under Apache 2.0 license as described in the file LICENSE.
+Authors: Jeremy Avigad
+
+The syntax of simple type theory, i.e. inductive definitions of types and terms.
+
+Notes:
+
+When it comes to basic types, type constructors, and constants, we distinguish between "built in"
+and "user" objects. The former are fixed for the implementation, and the implementation can refer
+to them directly (for example, logical connectives, arithmetic symbols, types like nat and bool,
+and type constructors like list, sum, and prod).
+
+TODO: objects store all the relevant information for type checking, but also information as to 
+the source. We can add additional predicates to say that a type or term is correct with respect
+to the environment, i.e. that the objects have the properties the terms say they have.
+
+TODO: In addition to "built in" and "user" objects, we can add "local" objects. In the meanwhile,
+we use indices everywhere.
+
+TODO: For now, we won't handle polymorphic types, though we will eventually (mostly following
+HOL light).
+
+TODO: For now, use naive equality tests. We can worry about more efficient tests (e.g. with
+unique id's) later, if necessary.
+
+TODO: if we replace each `= tt` by a coercion to bool, things break in some places. They are fixable,
+but then something more dramatic breaks in fol.syntax and the terms are huge.
+-/
+import data.list
+
+/- TODO: move these -/
+
+@[simp]
+theorem if_neg_eq {α : Type*} (p : Prop) [decidable p] (a b : α) : 
+  (if ¬ p then a else b) = (if p then b else a) :=
+begin
+  by_cases h : p; simp [h],
+end
+
+theorem to_bool_eq_to_bool (p q : Prop) [decidable p] [decidable q] :
+  (to_bool p = to_bool q) ↔ (p ↔ q) :=
+by by_cases p; simp [h]
+
+namespace list
+
+@[simp]
+theorem not_cons_prefix_nil {α : Type*} (a : α) (l : list α) : ¬ a :: l <+: nil :=
+by { unfold is_prefix, intro h, cases h, contradiction }
+
+@[simp]
+theorem cons_prefix_cons {α : Type*} (a₁ a₂ : α) (l₁ l₂ : list α) :
+  a₁ :: l₁ <+: a₂ :: l₂ ↔ a₁ = a₂ ∧ l₁ <+: l₂ :=
+begin
+  unfold is_prefix, 
+  split; intro h,
+  { cases h with l h, split, apply head_eq_of_cons_eq h, existsi l, apply tail_eq_of_cons_eq h},
+  cases h with h₀ h₁, cases h₁ with l h₁,
+  existsi l, rw [h₀, ← h₁], simp  
+end
+
+theorem length_le_of_prefix {α : Type*} {l₁ l₂ : list α} (h : l₁ <+: l₂) : length l₁ ≤ length l₂ :=
+length_le_of_sublist $ sublist_of_prefix h
+
+theorem drop_succ {α : Type*} (n : nat) (l : list α) : drop n.succ l = drop n (drop 1 l) :=
+by induction l; simp
+
+theorem drop_add {α : Type*} (n m : nat) (l : list α) : drop (n + m) l = drop n (drop m l) :=
+begin
+  revert l,
+  induction m with m ih, simp,
+  simp [nat.add_succ], intro l, rw drop_succ m, rw drop_succ (n + m), rw ih  
+end
+
+theorem drop_eq_nil  {α : Type*} (n : nat) (l : list α) : drop n l = [] ↔ n ≥ l.length:=
+begin
+  revert n,  
+  induction l with a l ih; simp, 
+  { apply nat.zero_le }, 
+  intro n, cases n with n; simp, 
+  { rw add_comm, apply nat.zero_lt_succ },
+  rw ih, rw [add_comm, ge, ge, nat.succ_le_succ_iff]
+end
+
+end list
+
+namespace hol
+
+/-
+Instead of option, we'll have failure produce error messages. But we will not use
+the full-blown exception monad or do anything fancy, to make it easier to reason
+about these programs.
+
+TODO: not using this yet.
+-/
+
+inductive except (α : Type*)
+| ok   : α → except
+| fail : string → except
+
+/- 
+    Types    
+-/
+
+namespace type
+
+  /- basic types -/
+
+  @[derive has_reflect, derive decidable_eq]
+  inductive basic : Type
+  | user : ℕ → basic
+  | prop 
+  | nat
+  | int
+  | bool
+  | unit
+
+  namespace basic
+    def repr : basic → string
+    | (user n) := "(basic.user " ++ n.repr ++ ")"
+    | prop := "basic.prop"
+    | nat  := "basic.nat"
+    | int  := "basic.int"
+    | bool := "basic.bool"
+    | unit := "basic.unit"
+
+    instance : has_repr basic := ⟨repr⟩   
+  end basic
+
+  /- type constructors -/
+
+  namespace constructor
+    @[derive has_reflect, derive decidable_eq]
+    inductive kind
+    | user : nat → kind
+    | list 
+    | prod 
+    | sum
+  end constructor
+
+  @[derive has_reflect, derive decidable_eq]
+  structure constructor :=
+  (symb : constructor.kind) (arity : nat)
+
+  namespace constructor
+    def user (n arity : nat)  : constructor := ⟨kind.user n, arity⟩
+    def list : constructor := ⟨kind.list, 1⟩ 
+    def prod : constructor := ⟨kind.prod, 2⟩ 
+    def sum : constructor := ⟨kind.sum, 2⟩ 
+    
+    def repr : constructor → string
+    | ⟨kind.user n, a⟩ := "(constructor.user " ++ n.repr ++ " " ++ a.repr ++")"
+    | ⟨kind.list, _⟩   := "constructor.list"   
+    | ⟨kind.prod, _⟩   := "constructor.list"   
+    | ⟨kind.sum, _⟩    := "constructor.list"
+
+    instance : has_repr constructor := ⟨repr⟩   
+  end constructor
+
+end type
+
+/- 
+The types themselves
+
+Notes:
+
+To avoid a nested inductive type, we'll use iterated application for constructors.
+
+Basic and arrow types are really special cases of constructors, but we'll keep them separate.
+-/
+
+@[derive has_reflect, derive decidable_eq]
+inductive type
+| Var         : nat → type
+| Basic       : hol.type.basic → type
+| Arr         : type → type → type
+| Constructor : hol.type.constructor → type
+| App         : type → type → type
+
+namespace type
+
+def repr : type → string
+| (Var n)         := "(Var " ++ n.repr ++ ")"
+| (Basic b)       := "(Basic " ++ b.repr ++ ")"
+| (Arr t₁ t₂)     := "(Arr " ++ t₁.repr ++ " " ++ t₂.repr ++")"
+| (Constructor c) := "(Constructor " ++ c.repr ++ ")"
+| (App t₁ t₂)     := "(App " ++ t₁.repr ++ " " ++ t₂.repr ++ ")"
+
+instance : has_repr type := ⟨repr⟩
+
+-- `arities_ok t l` says the type `t` iteratively applied to `l` makes sense
+def arities_ok_aux : type → list type → bool
+| (Var n)         l := l.empty
+| (Basic b)       l := l.empty
+| (Arr t₁ t₂)     l := arities_ok_aux t₁ l && arities_ok_aux t₂ l && l.empty
+| (Constructor c) l := c.arity = l.length
+| (App t₁ t₂)     l := arities_ok_aux t₂ [] && arities_ok_aux t₁ (t₂ :: l)
+
+def arities_ok (t : type) : bool := arities_ok_aux t []
+
+/-- Returns the domain of an arrow type, or the type itself if it is not an arrow. -/
+@[simp]
+def domain : type → type
+| (type.Arr t₁ t₂) := t₁
+| t                := t
+
+/-- Returns the codomain of an arrow type, or the type itself if it is not an arrow. -/
+@[simp]
+def codomain : type → type
+| (type.Arr t₁ t₂) := t₂ 
+| t                := t
+
+@[simp]
+def get_arg_types : type → list type
+| (type.Arr t₁ t₂) := t₁ :: get_arg_types t₂
+| _                := []
+
+@[simp]
+def num_arg_types : type → nat
+| (type.Arr t₁ t₂) := num_arg_types t₂ + 1
+| _                := 0
+
+lemma length_get_arg_types (t : type) : t.get_arg_types.length = t.num_arg_types :=
+by induction t; simp [*]
+
+@[simp]
+def get_return_type : type → type 
+| (type.Arr t₁ t₂) := get_return_type t₂
+| t                := t
+
+@[simp]
+def mk_fn_type : list type → type → type 
+| []        ret := ret
+| (a :: as) ret := (type.Arr a (mk_fn_type as ret))
+
+theorem mk_fn_type_eq (t : type) : t = mk_fn_type (get_arg_types t) (get_return_type t) :=
+by { induction t; simp [get_arg_types, get_return_type, mk_fn_type], assumption }
+
+@[simp]
+theorem get_return_type_codomain (t : type) : get_return_type (t.codomain) = get_return_type t :=
+by induction t; simp
+
+theorem get_arg_types_codomain (t : type) : get_arg_types (t.codomain) = t.get_arg_types.drop 1 :=
+by induction t; simp
+
+@[simp]
+def is_arrow : type → bool
+| (Arr t₁ t₂) := tt
+| _           := ff
+
+theorem is_arrow_mk_fn_type (ts : list type) (t : type) (h : t.is_arrow = ff) :
+  (mk_fn_type ts t).is_arrow = (ts ≠ []) :=
+by induction ts; simp [h]
+
+theorem is_arrow_get_return_type_eq_ff (t : type) : t.get_return_type.is_arrow = ff :=
+by induction t; simp [*]
+
+theorem eq_of_is_arrow (t : type) (h : is_arrow t = tt) : t = Arr (domain t) (codomain t) :=
+by cases t; simp at h; trivial
+
+lemma cons_prefix_get_arg_types (ty ty' : type) (tys : list type) :
+  (ty :: tys) <+: ty'.get_arg_types ↔ 
+    is_arrow ty' = tt ∧ ty = ty'.domain ∧ tys <+: ty'.codomain.get_arg_types :=
+by cases ty'; simp
+
+end type
+
+/- convenient type constructors -/
+
+section
+open type
+
+def mk_prop := Basic basic.prop
+def mk_nat := Basic basic.nat
+def mk_int := Basic basic.int
+def mk_unit := Basic basic.int
+def mk_bool := Basic basic.bool
+def mk_user_type (n : ℕ) := Basic (basic.user n)
+
+def mk_list_type (t : type) : type := App (Constructor constructor.list) t
+def mk_prod_type (t₁ t₂ : type) : type := App (App (Constructor constructor.prod) t₁) t₂
+def mk_sum_type (t₁ t₂ : type) : type := App (App (Constructor constructor.sum) t₁) t₂
+
+--notation t₁ ` ⇒ `:65 t₂ := Arr t₁ t₂  
+infixr ` ⇒ ` := Arr
+
+theorem arities_ok_mk_prop : arities_ok mk_prop :=
+by simp [mk_prop, arities_ok, arities_ok_aux, list.empty]
+
+theorem arities_ok_mk_nat : arities_ok mk_nat :=
+by simp [mk_nat, arities_ok, arities_ok_aux, list.empty]
+
+theorem arities_ok_mk_int : arities_ok mk_int :=
+by simp [mk_int, arities_ok, arities_ok_aux, list.empty]
+
+theorem arities_ok_mk_list_type (t : type) (h : arities_ok t = tt) : 
+  arities_ok (mk_list_type t) = tt :=
+by { simp [arities_ok] at *, simp [mk_list_type, arities_ok_aux, h, constructor.list] }
+
+theorem arities_ok_mk_prod_type (t₁ t₂ : type) 
+    (h₁ : arities_ok t₁ = tt) (h₂ : arities_ok t₂ = tt) : 
+  arities_ok (mk_prod_type t₁ t₂) = tt :=
+by { simp [arities_ok] at *, simp [mk_prod_type, arities_ok_aux, h₁, h₂, constructor.prod] }
+
+theorem arities_ok_mk_sum_type (t₁ t₂ : type) 
+    (h₁ : arities_ok t₁ = tt) (h₂ : arities_ok t₂ = tt) : 
+  arities_ok (mk_sum_type t₁ t₂) = tt :=
+by { simp [arities_ok] at *, simp [mk_sum_type, arities_ok_aux, h₁, h₂, constructor.sum] }
+
+end
+
+/-
+    Terms
+-/
+
+namespace term
+
+  /- constants -/
+
+  namespace const
+    @[derive has_reflect, derive decidable_eq]
+    inductive kind
+    | user : nat → kind
+    | true 
+    | false 
+    | not
+    | and
+    | or
+    | implies
+    | iff
+    | all
+    | ex
+    | add
+    | mul
+    | sub
+    | bval : bool → kind
+    | nval : nat → kind
+  end const
+
+  -- instantiations are for polymorphic constants
+  @[derive has_reflect, derive decidable_eq]
+  structure const :=
+  (symb : const.kind) (type : type) (insts : list hol.type)
+
+  namespace const
+    def user (n : nat) (t : hol.type) (l : list hol.type) : const := ⟨kind.user n, t, l⟩
+    def true : const := ⟨kind.true, mk_prop, []⟩ 
+    def false : const := ⟨kind.false, mk_prop, []⟩ 
+    def not : const := ⟨kind.not, mk_prop ⇒ mk_prop, []⟩
+    def and : const := ⟨kind.and, mk_prop ⇒ (mk_prop ⇒ mk_prop), []⟩
+    def or : const := ⟨kind.or, mk_prop ⇒ (mk_prop ⇒ mk_prop), []⟩
+    def implies : const := ⟨kind.implies, mk_prop ⇒ (mk_prop ⇒ mk_prop), []⟩
+    def iff : const := ⟨kind.iff, mk_prop ⇒ (mk_prop ⇒ mk_prop), []⟩
+    def add : const := ⟨kind.add, mk_nat ⇒ (mk_nat ⇒ mk_nat), []⟩
+    def mul : const := ⟨kind.mul, mk_nat ⇒ (mk_nat ⇒ mk_nat), []⟩
+    def sub : const := ⟨kind.sub, mk_nat ⇒ (mk_nat ⇒ mk_nat), []⟩
+    def tt  : const := ⟨kind.bval tt, mk_bool, []⟩
+    def ff  : const := ⟨kind.bval ff, mk_bool, []⟩
+    def nval (n : nat) : const := ⟨kind.nval n, mk_nat, []⟩
+
+    def repr : const → string
+    | ⟨kind.user n, t, l⟩       := "(const.user " ++ n.repr ++ " " ++ t.repr ++ " " ++ l.repr ++ ")"
+    | ⟨kind.true, _, _⟩         := "const.true"
+    | ⟨kind.false, _, _⟩        := "const.false"
+    | ⟨kind.not, _, _⟩          := "const.not"
+    | ⟨kind.and, _, _⟩          := "const.and"
+    | ⟨kind.or, _, _⟩           := "const.or"
+    | ⟨kind.implies, _, _⟩      := "const.implies"
+    | ⟨kind.iff, _, _⟩          := "const.iff"
+    | ⟨kind.all, _, _⟩          := "const.all"
+    | ⟨kind.ex, _, _⟩           := "const.ex"
+    | ⟨kind.add, _, _⟩          := "const.add"
+    | ⟨kind.mul, _, _⟩          := "const.mul"
+    | ⟨kind.sub, _, _⟩          := "const.sub"
+    | ⟨kind.bval bool.tt, _, _⟩ := "const.tt"
+    | ⟨kind.bval bool.ff, _, _⟩ := "const.ff"
+    | ⟨kind.nval n, _, _⟩       := "(const.nval " ++ n.repr ++ ")"
+
+    instance : has_repr const := ⟨repr⟩
+
+    def is_connective : const → bool
+    | ⟨kind.true, t, l⟩         := if t = mk_prop then l.empty else bool.ff
+    | ⟨kind.false, t, l⟩        := if t = mk_prop then l.empty else bool.ff
+    | ⟨kind.not, t, l⟩          := if t = (mk_prop ⇒ mk_prop) then l.empty else bool.ff
+    | ⟨kind.and, t, l⟩          := if t = (mk_prop ⇒ mk_prop ⇒ mk_prop) then l.empty else bool.ff
+    | ⟨kind.or, t, l⟩           := if t = (mk_prop ⇒ mk_prop ⇒ mk_prop) then l.empty else bool.ff
+    | ⟨kind.implies, t, l⟩      := if t = (mk_prop ⇒ mk_prop ⇒ mk_prop) then l.empty else bool.ff
+    | ⟨kind.iff, t, l⟩          := if t = (mk_prop ⇒ mk_prop ⇒ mk_prop) then l.empty else bool.ff
+    | _                         := bool.ff
+  end const
+
+end term
+
+/- the terms themselves -/
+
+@[derive has_reflect, derive decidable_eq]
+inductive term
+| Var     : nat → term
+| Const   : hol.term.const → term
+| App     : term → term → term                -- application
+| Abs     : string → hol.type → term → term   -- the string gives the preferred name
+
+namespace term
+
+def sizeof' : term → nat
+| (Var n)      := 0
+| (Const n)    := 0
+| (App s t)    := sizeof' s + sizeof' t + 1
+| (Abs s ty t) := sizeof t + 1
+
+instance : has_sizeof term := ⟨sizeof'⟩
+
+def repr : term → string
+| (Var n)      := "(Var " ++ n.repr ++ ")"
+| (Const c)    := "(Const " ++ c.repr ++ ")"
+| (App t₁ t₂)  := "(App " ++ t₁.repr ++ t₂.repr ++ ")"
+| (Abs s ty t) := "(Abs " ++ _root_.repr s ++ " " ++ ty.repr ++ " " ++ t.repr ++ ")"
+
+/-- Inter the type of a term, given an assignment to free variables. Assumes the expression is well-typed-/
+def typeof : term → list type → type
+| (Var n) σ       := if h : n < σ.length then σ.nth_le n h else mk_nat
+| (Const c) σ     := c.type
+| (App t₁ t₂) σ   := (typeof t₁ σ).codomain
+| (Abs s ty t) σ  := ty ⇒ typeof t (ty :: σ)
+
+inductive is_well_typed : term → list type → Prop
+| wt_var (n : ℕ) (σ : list type) (h : n < σ.length)      : is_well_typed (Var n) σ
+| wt_const (c : const) (σ : list type)                   : is_well_typed (Const c) σ
+| wt_app (t₁ t₂ : term) (σ : list type) 
+    (h₁ : is_well_typed t₁ σ) 
+    (h₂ : is_well_typed t₂ σ) 
+    (h₃ : (typeof t₁ σ).is_arrow = tt) 
+    (h₄ : (typeof t₁ σ).domain = typeof t₂ σ)            : is_well_typed (App t₁ t₂) σ
+| wt_abs (s : string) (ty : type) (t : term) 
+      (σ : list type)
+    (h₁ : is_well_typed t (ty :: σ))                     : is_well_typed (Abs s ty t) σ
+
+/-- Inter the type of a term, given an assignment to free variables. Returns none of expression is not well-typed. -/
+def typeof_p : term → list type → option type 
+| (Var n)     σ  := σ.nth n
+| (Const c)   σ  := some c.type 
+| (App t₁ t₂) σ  := 
+    match typeof_p t₁ σ, typeof_p t₂ σ with 
+    | (some (type.Arr u v)), (some w) := if u = w then some v else none
+    | _                    , _        := none
+    end
+| (Abs s ty t) σ := match typeof_p t (ty :: σ) with
+                    | some ty₂ := some (type.Arr ty ty₂)
+                    | _        := none
+                    end
+
+@[simp]
+def is_var : term → bool
+| (Var n) := tt
+| _       := ff
+
+def var_num : term → nat
+| (Var n) := n
+| _       := 0
+
+@[simp]
+def is_const : term → bool
+| (Const c) := tt
+| _         := ff
+
+@[simp]
+def is_app : term → bool
+| (App f a) := tt
+| _         := ff
+
+def app_fn : term → term
+| (App f a) := f
+| t         := t
+
+def app_arg : term → term
+| (App f a) := a
+| t         := t
+
+@[simp]
+def get_app_fn : term → term
+| (App f a) := get_app_fn f
+| t          := t
+
+def get_app_num_args : term → ℕ 
+| (App f a) := get_app_num_args f + 1
+| t         := 0
+
+def get_app_args_aux : term → list term → list term
+| (App t₁ t₂)  args := get_app_args_aux t₁ (t₂ :: args)
+| (Var n)      args := args
+| (Const c)    args := args
+| (Abs s ty t) args := args
+
+def get_app_args (t : term) : list term := get_app_args_aux t []
+
+@[simp]
+def mk_app : term → list term → term
+| t []       := t
+| t (a::as)  := mk_app (App t a) as
+
+theorem mk_app_get_app_aux (t : term) : 
+  ∀ as, mk_app (get_app_fn t) (get_app_args_aux t as) = mk_app t as :=
+by induction t; simp [get_app_fn, get_app_args_aux, mk_app, *]
+
+theorem mk_app_get_app (t : term) : mk_app (get_app_fn t) (get_app_args t) = t :=
+by simp [get_app_args, mk_app_get_app_aux, mk_app]
+
+@[simp]
+def is_well_typed_b : term → list type → bool
+| (Var n)     σ := if n < σ.length then tt else ff
+| (Const c)   σ := tt
+| (App t₁ t₂) σ := is_well_typed_b t₁ σ && is_well_typed_b t₂ σ && 
+                     (typeof t₁ σ).is_arrow && ((typeof t₁ σ).domain = typeof t₂ σ)
+| (Abs s ty t) σ := is_well_typed_b t (ty :: σ)
+
+theorem is_well_typed_iff (t : term) : 
+  ∀ σ, is_well_typed t σ ↔ (is_well_typed_b t σ = tt) :=
+begin
+  induction t with _ _ _ _ h₁ h₂ _ ty _ h,
+  {intro σ, split, {intro h, cases h; simp [*]}, intro h, simp at h, constructor, assumption},
+  {intro σ, split, {intro h, cases h; simp [*]}, intro h, simp at h, constructor},
+  {intro σ, simp [(h₁ σ).symm, (h₂ σ).symm], split, {intro h, cases h; simp [*]}, intro h, constructor; simp [*]},
+  {intro σ, simp [(h (ty::σ)).symm], split, {intro h, cases h, assumption}, 
+    intro h, constructor; simp [*]}
+end
+
+theorem is_well_typed_mk_app (l : list term) (σ : list type) :
+  ∀ t, is_well_typed (mk_app t l) σ ↔ 
+         is_well_typed t σ ∧ (∀ t' ∈ l, is_well_typed t' σ) ∧ 
+           l.map (λ t', typeof t' σ) <+: (t.typeof σ).get_arg_types :=
+begin
+  induction l with t' l' ih,
+  { simp [list.nil_prefix] },
+  simp, intro t, rw [ih (App t t')], simp [is_well_typed_iff],
+  split, 
+  { intro h, simp [*, typeof] at *,
+    rcases h with ⟨⟨h₀, h₁, h₂, h₃⟩, h₄, h₅⟩,  
+    split, exact h₄, rw [type.eq_of_is_arrow _ h₂],
+    simp, rw [h₃], simp, exact h₅},
+  intro h, rcases h with ⟨h,  ⟨h₀, h₁⟩, h₂⟩,
+  have h₃ := (type.cons_prefix_get_arg_types _ _ _).mp h₂,
+  rcases h₃ with ⟨h₃, h₄, h₅⟩,
+  simp [h, h₀, h₁, h₃, h₄, h₅, typeof],
+  assumption  
+end
+
+theorem typeof_mk_app (t: term) (as : list term) (σ : list type) :
+  typeof (mk_app t as) σ = 
+    type.mk_fn_type (((t.typeof σ).get_arg_types).drop (as.length)) 
+      (t.typeof σ).get_return_type :=
+begin
+  revert t, 
+  induction as with a as ih, 
+  { intro t, simp, rw ← type.mk_fn_type_eq (t.typeof σ) },
+  intro t, simp, rw (ih (App t a)), simp [typeof], rw [add_comm, list.drop_add],
+  simp [type.get_arg_types_codomain]
+end
+
+theorem typeof_mk_app_is_arrow (t: term) (as : list term) (σ : list type) :
+  (typeof (mk_app t as) σ).is_arrow = (as.length < (t.typeof σ).num_arg_types) := 
+begin
+  rw [typeof_mk_app, type.is_arrow_mk_fn_type, to_bool_eq_to_bool, ne, list.drop_eq_nil,
+    lt_iff_not_ge, type.length_get_arg_types], --simp [- bool.to_bool_not],
+  apply type.is_arrow_get_return_type_eq_ff
+end
+
+theorem length_le_num_arg_types_typeof  {t: term} {as : list term} {σ : list type} 
+    (h : is_well_typed (mk_app t as) σ) :
+  as.length ≤ (t.typeof σ).num_arg_types :=
+begin
+  have : as.map (λ t', typeof t' σ) <+: (t.typeof σ).get_arg_types, 
+    from ((is_well_typed_mk_app as σ t).mp h).right.right,
+  have := list.length_le_of_prefix this,
+  simpa [type.length_get_arg_types]
+end
+
+theorem length_get_app_args_of_not_is_arrow {t : term} {σ : list type} 
+    (h : (t.typeof σ).is_arrow = ff) (h' : t.is_well_typed σ) :
+  t.get_app_args.length = (t.get_app_fn.typeof σ).num_arg_types :=
+begin
+  rw ← mk_app_get_app t at h h',
+  have : t.get_app_args.length ≤ (t.get_app_fn.typeof σ).num_arg_types,
+    from length_le_num_arg_types_typeof h',
+  by {apply le_antisymm this, rw typeof_mk_app_is_arrow at h, simp at h, exact h }
+end
+
+theorem get_arg_types_typeof_get_app_fn {t : term} {σ : list type} 
+    (h : (t.typeof σ).is_arrow = ff) (h' : t.is_well_typed σ) :
+  (t.get_app_fn.typeof σ).get_arg_types = t.get_app_args.map (λ t', t'.typeof σ) :=
+begin
+  have : t.get_app_args.length = (t.get_app_fn.typeof σ).num_arg_types,
+    from length_get_app_args_of_not_is_arrow h h',
+  rw ← mk_app_get_app t at h h',
+  have : t.get_app_args.map (λ t', typeof t' σ) <+: (t.get_app_fn.typeof σ).get_arg_types, 
+    from ((is_well_typed_mk_app t.get_app_args σ t.get_app_fn).mp h').right.right,
+  have : t.get_app_args.map (λ t', typeof t' σ) = (t.get_app_fn.typeof σ).get_arg_types,
+    by { apply list.eq_of_prefix_of_length_eq this, rw type.length_get_arg_types, simp, assumption},
+  exact this.symm
+end
+
+theorem typeof_eq_of_not_is_arrow {t : term} {σ : list type} 
+    (h : (t.typeof σ).is_arrow = ff) (h' : t.is_well_typed σ) :
+  t.typeof σ = ((t.get_app_fn).typeof σ).get_return_type :=
+begin
+  have h₀ : t.typeof σ = (mk_app t.get_app_fn t.get_app_args).typeof σ,
+    by rw mk_app_get_app,
+  transitivity, exact h₀,
+  rw [typeof_mk_app, length_get_app_args_of_not_is_arrow h h', ← type.length_get_arg_types],
+  rw (list.drop_eq_nil _ _).mpr, simp, apply le_refl
+end
+
+end term
+
+end hol
